Switch Pf to build substs into axiom calls. Eliminate dependencies on old versions.

src/named/Pf.v
@@ -18,24 +18,7 @@ Inductive pf : Set :=
 (* congruence for constructors *)
 | pcon : string -> list pf -> pf
 (* appealing to a language axiom *)
-| ax : string -> pf
-(* applying a substitution;
-   can't be distributed over axioms
-   unless in the context of a given language
-   
-   TODO: use a named list or regular list?
-   Can I figure out appropriate names given the language?
-   Not in the var case. Should I add a ctx argument to
-   the var case? Seems like it might be a good idea.
-   A relevant is how these terms will be checked.
-   I'll leave this consideration until I get to my proves_wf function.
-
-   TODO: do I want this or no?
-   Might be able to eliminate it, but probably
-   not worth it at the moment.
- *)
-| sub : pf -> ctx (*TODO: hack to beat fixpoint checker; remove when able*) ->
-        named_list_set pf (* interface ctx wf*) -> list pf (* subst le *) -> pf
+| ax : string -> list pf -> pf
 | sym : pf -> pf
 | trans : pf -> pf -> pf
 | conv : pf (*term*) -> pf (*sort*) -> pf.
@@ -50,12 +33,8 @@ Fixpoint pf_ind
          (IHC : forall n l,
              List.fold_right (fun t => and (P t)) True l ->
              P (pcon n l))
-         (IHA : forall n, P(ax n))
-         (IHS : forall e' c pfc l,
-             P e' ->
-             List.fold_right (fun p => and (P p.2)) True pfc ->
-             List.fold_right (fun p => and (P p)) True l ->
-             P (sub e' c pfc l))
+         (IHA : forall n pfs, 
+             List.fold_right (fun p => and (P p)) True pfs -> P(ax n pfs))
          (IHSY : forall e', P e' -> P (sym e'))
          (IHT : forall e1 e2,
              P e1 -> P e2 -> P (trans e1 e2))
@@ -68,30 +47,24 @@ Fixpoint pf_ind
     let fix loop l :=
         match l return List.fold_right (fun t => and (P t)) True l with
         | [::] => I
-        | e' :: l' => conj (pf_ind IHV IHC IHA IHS IHSY IHT IHCV e') (loop l')
+        | e' :: l' => conj (pf_ind IHV IHC IHA IHSY IHT IHCV e') (loop l')
         end in
     IHC n l (loop l)
-  | ax n => IHA n
-  | sub e' c pfc l =>
-    let fix cloop l :=
-        match l return List.fold_right (fun t => and (P t.2)) True l with
-        | [::] => I
-        | (_,e') :: l' => conj (pf_ind IHV IHC IHA IHS IHSY IHT IHCV e') (cloop l')
-        end in
+  | ax n pfs => 
     let fix loop l :=
         match l return List.fold_right (fun t => and (P t)) True l with
         | [::] => I
-        | e' :: l' => conj (pf_ind IHV IHC IHA IHS IHSY IHT IHCV e') (loop l')
+        | e' :: l' => conj (pf_ind IHV IHC IHA IHSY IHT IHCV e') (loop l')
         end in
-    IHS e' c pfc l (pf_ind IHV IHC IHA IHS IHSY IHT IHCV e') (cloop pfc) (loop l)
+    IHA n pfs (loop pfs)
   | sym e' =>
-    IHSY e' (pf_ind IHV IHC IHA IHS IHSY IHT IHCV e')
+    IHSY e' (pf_ind IHV IHC IHA IHSY IHT IHCV e')
   | trans e1 e2 =>
-    IHT e1 e2 (pf_ind IHV IHC IHA IHS IHSY IHT IHCV e1)
-        (pf_ind IHV IHC IHA IHS IHSY IHT IHCV e2)
+    IHT e1 e2 (pf_ind IHV IHC IHA IHSY IHT IHCV e1)
+        (pf_ind IHV IHC IHA IHSY IHT IHCV e2)
   | conv e1 e2 =>
-    IHCV e1 e2 (pf_ind IHV IHC IHA IHS IHSY IHT IHCV e1)
-        (pf_ind IHV IHC IHA IHS IHSY IHT IHCV e2)
+    IHCV e1 e2 (pf_ind IHV IHC IHA IHSY IHT IHCV e1)
+        (pf_ind IHV IHC IHA IHSY IHT IHCV e2)
   end.
 
 (* TODO
@@ -164,13 +137,9 @@ Section RuleChecking.
            al1 <- get_subseq args (with_names_from c' el1);
            al2 <- get_subseq args (with_names_from c' el2);
            ret (scon name (map snd al1), scon name (map snd al2))
-      | ax name =>
+      | ax name pfs =>
         do (sort_le c' e1 e2) <- named_list_lookup_err l name;
-           ! c == c';
-           ret (e1,e2)
-      | sub p c' _ pl =>
-        do (e1, e2) <- synth_le_sort p c';
-           (el1, el2) <- synth_le_args pl c c';
+           (el1, el2) <- synth_le_args pfs c c';
            let s1 := with_names_from c' el1;
            let s2 := with_names_from c' el2;
            ret (e1[/s1/],e2[/s2/])
@@ -183,35 +152,53 @@ Section RuleChecking.
            !e2 == e2';
            ret (e1,e3)
       | conv pt p => None
-  end.
+    end.
 
-    Fixpoint synth_le_sort_ex (pt : pf) (c : ctx) : option (sort * sort) :=
-      match pt with
-      | pvar x => None
-      | pcon name pl =>
-        do (sort_rule c' args) <- named_list_lookup_err l name;
-           (el1, el2) <- synth_le_args pl c c';
-           ret (scon name el1, scon name el2)
-      | ax name =>
-        do (sort_le c' e1 e2) <- named_list_lookup_err l name;
-           ! c == c';
-           ret (e1,e2)
-      | sub p c' _ pl =>
-        do (e1, e2) <- synth_le_sort p c';
-           (el1, el2) <- synth_le_args pl c c';
-           let s1 := with_names_from c' el1;
-           let s2 := with_names_from c' el2;
-           ret (e1[/s1/],e2[/s2/])
-      | sym p =>
-        do (e1,e2) <- synth_le_sort_ex p c;
-           ret (e2,e1)
-      | trans p1 p2 =>
-        do (e1,e2) <- synth_le_sort_ex p1 c;
-           (e2',e3) <- synth_le_sort_ex p2 c;
-           !e2 == e2';
-           ret (e1,e3)
-      | conv pt p => None
-    end.    
+    Lemma synth_le_args_size_l l0 l1 l2 c c0
+      : Some (l1, l2) = synth_le_args l0 c c0 ->
+        size l1 = size c0.
+    Proof.
+      revert l1 l2 c0.
+      induction l0; intros; destruct c0; break; simpl in *; try by (inversion H; subst; auto).
+      revert H.
+      case_match; [| intro H; inversion H];
+        break.
+      case_match; [| intro H; inversion H];
+        break.
+      case_match; [| intro H; inversion H];
+        break.
+      symmetry in HeqH1.
+      case.
+      move: HeqH1 => /eqP.
+      intros.
+      subst.
+      simpl.
+      f_equal; eauto.
+    Qed.
+
+    Lemma synth_le_args_size_r l0 l1 l2 c c0
+      : Some (l1, l2) = synth_le_args l0 c c0 ->
+        size l2 = size c0.
+    Proof.
+      revert l1 l2 c0.
+      induction l0; intros; destruct c0; break; simpl in *; try by (inversion H; subst; auto).
+      revert H.
+      case_match; [| intro H; inversion H];
+        break.
+      case_match; [| intro H; inversion H];
+        break.
+      case_match; [| intro H; inversion H];
+        break.
+      symmetry in HeqH1.
+      case.
+      move: HeqH1 => /eqP.
+      intros.
+      subst.
+      simpl.
+      f_equal; eauto.
+    Qed.
+
+
   End InnerLoop.
 
   (* Defined over proof and implicit terms
@@ -228,16 +215,12 @@ Section RuleChecking.
          al2 <- get_subseq args (with_names_from c' el2);
          ret (t[/with_names_from c' el2/],
               con name (map snd al1), con name (map snd al2))
-    | ax name =>
-      do (term_le c' e1 e2 t) <- named_list_lookup_err l name;
-         !c == c';
-         ret (t,e1,e2)
-    | sub p' c' _ pl =>
-      do (t,e1, e2) <- synth_le_term p' c';
-         (el1, el2) <- synth_le_args synth_le_term pl c c';
-         let s1 := with_names_from c' el1;
-         let s2 := with_names_from c' el2;
-         ret (t[/s2/],e1[/s1/],e2[/s2/])
+      | ax name pfs =>
+        do (term_le c' e1 e2 t) <- named_list_lookup_err l name;
+           (el1, el2) <- synth_le_args synth_le_term pfs c c';
+           let s1 := with_names_from c' el1;
+           let s2 := with_names_from c' el2;
+           ret (t[/s2/],e1[/s1/],e2[/s2/])
     | sym p' =>
       do (t,e1,e2) <- synth_le_term p' c;
          ret (t,e2,e1)
@@ -254,236 +237,15 @@ Section RuleChecking.
          ret (t1,e1,e2)
   end.
 
-  Fixpoint synth_le_term_ex (p : pf) (c : ctx) {struct p}
-    : option (sort*exp*exp) :=
-    match p with
-    | pvar x =>
-      do t <- named_list_lookup_err c x;
-         ret (t,var x, var x)
-    | pcon name pl =>
-      do (term_rule c' args t) <- named_list_lookup_err l name;
-         (el1, el2) <- synth_le_args synth_le_term_ex pl c c';
-         ret (t[/with_names_from c' el2/],
-              con name el1, con name el2)
-    | ax name =>
-      do (term_le c' e1 e2 t) <- named_list_lookup_err l name;
-         !c == c';
-         ret (t,e1,e2)
-    | sub p' c' _ pl =>
-      do (t,e1, e2) <- synth_le_term_ex p' c';
-         (el1, el2) <- synth_le_args synth_le_term_ex pl c c';
-         let s1 := with_names_from c' el1;
-         let s2 := with_names_from c' el2;
-         ret (t[/s2/],e1[/s1/],e2[/s2/])
-    | sym p' =>
-      do (t,e1,e2) <- synth_le_term_ex p' c;
-         ret (t,e2,e1)
-    | trans p1 p2 =>
-      do (t,e1,e2) <- synth_le_term_ex p1 c;
-         (t',e2',e3) <- synth_le_term_ex p2 c;
-         ! t == t';
-         ! e2 == e2';
-         ret (t,e1,e3)
-    | conv pt p' =>
-      do (t, e1, e2) <- synth_le_term_ex p' c;
-         (t', t1) <- synth_le_sort_ex synth_le_term_ex pt c;
-         ! t == t';
-         ret (t1,e1,e2)
-  end.
-
-  Section InnerLoop.
-    Context (synth_wf_term : pf -> ctx -> option (sort*exp)).
-
-    Fixpoint synth_wf_args (pl : list pf) (c c' : ctx) {struct pl}
-      : option (list exp) :=
-      match pl with
-      | [::] => do [::] <- do ret c'; ret ([::])
-      | p::pl' =>
-        do (_,t)::c'' <- do ret c';
-           (t',e) <- synth_wf_term p c;
-           el <- synth_wf_args pl' c c'';
-           ! t' == t[/with_names_from c'' el/];
-           ret (e::el)
-     end.
-  End InnerLoop.
-
-  (* Defined over proof and implicit terms
-   *)
-  Fixpoint synth_wf_term (p : pf) (c : ctx) {struct p} : option (sort*exp) :=
-    match p with
-    | pvar x =>
-      do t <- named_list_lookup_err c x;
-         ret (t,var x)
-    | pcon name pl =>
-      do (term_rule c' args t) <- named_list_lookup_err l name;
-         el <- synth_wf_args synth_wf_term pl c c';
-         al <- get_subseq args (with_names_from c' el);
-         ret (t[/with_names_from c' el/], con name (map snd al))
-    | ax name => None
-    | sub p' c' _ pl => None
-    | sym p' => None
-    | trans p1 p2 => None
-    | conv pt p' =>
-      do (t, e) <- synth_wf_term p' c;
-         (t', t1) <- synth_le_sort synth_le_term pt c;
-         ! t == t';
-         ret (t1,e)
-  end.
-
-  Definition synth_wf_sort (pt : pf) (c : ctx) : option sort :=
-      match pt with
-      | pvar x => None
-      | pcon name pl =>
-        do (sort_rule c' args) <- named_list_lookup_err l name;
-           el <- synth_wf_args synth_wf_term pl c c';
-           al <- get_subseq args (with_names_from c' el);
-           ret (scon name (map snd al))
-      | ax name => None
-      | sub p c' _ pl => None
-      | sym p => None
-      | trans p1 p2 => None
-      | conv pt p => None
-    end.
-
-  Fixpoint synth_wf_ctx pl : option ctx :=
-    match pl with
-    | [::] => do ret [::]
-    | (name,p)::pl' =>
-      do c' <- synth_wf_ctx pl';
-         ! fresh name c';
-         t <- synth_wf_sort p c';
-         ret (name,t)::c'
-  end.
-
-  Fixpoint all_ctxs_ok p : bool :=
-    match p with
-    | pvar _ => true
-    | pcon _ pl => foldr andb true (map all_ctxs_ok pl)
-    | ax name => true
-    | sub p c' plc pl =>
-      (Some c' == synth_wf_ctx plc) &&
-      (foldr andb true (map (fun q => (all_ctxs_ok q.2)) plc)) &&
-      (foldr andb true (map all_ctxs_ok pl))
-    | sym p => all_ctxs_ok p
-    | trans p1 p2 => (all_ctxs_ok p1) && (all_ctxs_ok p2)
-    | conv pt p => (all_ctxs_ok pt) && (all_ctxs_ok p)
-    end.
-
-  Definition list_all_ctxs_ok pl :=
-    foldr andb true (map all_ctxs_ok pl).
-
-  
-  Definition named_list_all_ctxs_ok (pl : named_list pf) :=
-    foldr andb true (map (fun p => all_ctxs_ok p.2) pl).
-
-  
-  Definition check_le_term p c t e1 e2 : bool :=
-    (Some (t,e1, e2) == synth_le_term p c) &&
-    (all_ctxs_ok p).
-  Arguments check_le_term p c t e1 e2/.
-  
-  Definition check_le_sort p c t1 t2 : bool :=
-    (Some (t1, t2) == synth_le_sort synth_le_term p c)&&
-    (all_ctxs_ok p).
-  Arguments check_le_sort p c t1 t2/.
-
-  
-  Definition check_le_args pl c c' el1 el2 : bool :=
-    (Some (el1, el2) == synth_le_args synth_le_term pl c c')&&
-    (list_all_ctxs_ok pl).
-  Arguments check_le_args pl c c' el1 el2/.
-
-  
-  Definition check_wf_term p c e t : bool :=
-    (Some (t,e) == synth_wf_term p c) &&
-    (all_ctxs_ok p).
-  Arguments check_wf_term p c e t/.
-  
-  Definition check_wf_sort p c t : bool :=
-    (Some t == synth_wf_sort p c) &&
-    (all_ctxs_ok p).
-  Arguments check_wf_sort p c t/.
-  
-  Definition check_wf_ctx pl c : bool :=
-    (Some c == synth_wf_ctx pl) &&
-    (named_list_all_ctxs_ok pl).
-  Arguments check_wf_ctx pl c/.
-
-  
-  Definition check_wf_args pl c el c' : bool :=
-    (Some el == synth_wf_args synth_wf_term pl c c')&&
-    (list_all_ctxs_ok pl).
-  Arguments check_wf_args pl c el c'/.
-  
-
-  Variant rule_pf : Set :=
-  | sort_rule_pf : named_list_set pf -> list string -> rule_pf
-  | term_rule_pf : named_list_set pf -> list string -> pf -> rule_pf
-  | sort_le_pf : named_list_set pf -> pf -> pf -> rule_pf
-  | term_le_pf : named_list_set pf -> pf -> pf -> pf (*sort; TODO: not needed*)-> rule_pf.
-      
-  Definition synth_wf_rule rp : option rule :=
-    match rp with
-    | sort_rule_pf pl args =>
-      do !named_list_all_ctxs_ok pl;
-         c <- synth_wf_ctx pl;
-         ! subseq args (map fst c);
-         ret sort_rule c args
-    | term_rule_pf pl args p =>
-      do !named_list_all_ctxs_ok pl;
-         !all_ctxs_ok p;
-         c <- synth_wf_ctx pl;
-         t <- synth_wf_sort p c;
-         ! subseq args (map fst c);
-         ret term_rule c args t
-    | sort_le_pf pl p1 p2 =>
-      do !named_list_all_ctxs_ok pl;
-         !all_ctxs_ok p1;
-         !all_ctxs_ok p2;
-         c <- synth_wf_ctx pl;
-         t1 <- synth_wf_sort p1 c;
-         t2 <- synth_wf_sort p2 c;
-         ret sort_le c t1 t2
-    | term_le_pf pl p1 p2 pt =>
-      do !named_list_all_ctxs_ok pl;
-         !all_ctxs_ok p1;
-         !all_ctxs_ok p2;
-         !all_ctxs_ok pt;
-         c <- synth_wf_ctx pl;
-         (t1,e1) <- synth_wf_term p1 c;
-         (t2,e2) <- synth_wf_term p2 c;
-         t <- synth_wf_sort p2 c;
-         ! t == t1;
-         ! t == t2;
-         ret term_le c e1 e2 t
-  end.
-
-  Definition check_wf_rule rp r : bool :=
-    Some r == synth_wf_rule rp.
-  Arguments check_wf_rule rp r/.
 
 End RuleChecking.
   
-Fixpoint synth_wf_lang rpl : option lang :=
-  match rpl with
-  | [::] => do ret [::]
-  | (name,rp)::rpl' =>
-    do l' <- synth_wf_lang rpl';
-       ! fresh name l';
-       r <- synth_wf_rule l' rp;
-       ret (name,r)::l'
-  end.
 
-Definition check_wf_lang rpl l : bool :=
-  Some l == synth_wf_lang rpl.
-Arguments check_wf_lang rpl l/.
+Lemma get_subseq_exact (s : subst)
+  : Some s = get_subseq (map fst s) s.
+Proof.
+  induction s; intros; break; simpl in *; auto.
+  rewrite ?eq_refl.
+  rewrite <-IHs; eauto.
+Qed.
 
-
-Arguments check_wf_args l pl c el c'/.
-Arguments check_wf_ctx l pl c/.
-Arguments check_wf_sort l p c t/.
-Arguments check_wf_term l p c e t/.
-Arguments check_le_args l pl c c' el1 el2/.
-Arguments check_le_sort l p c t1 t2/.
-Arguments check_le_term l p c t e1 e2/.
-Arguments check_wf_rule l rp r/.
