src/named/Exp.v
@@ -680,3 +680,34 @@ Module Notations.
   Check (as_ctx {{c "x" : #"env", "y" : #"ty" %"x", "z" : #"ty" %"x"}}).
 
 End Notations.
+
+
+
+Lemma with_names_from_args_subst (c':ctx) s' (s : list exp)
+  : with_names_from c' s[/s'/] = (with_names_from c' s)[/s'/].
+Proof using .
+  elim: c' s; intros until s; case: s; intros; break; simpl in *; auto.
+  f_equal; auto.
+  by fold_Substable.
+Qed.
+
+(* TODO: move to utils? need more general types to do so*)
+Lemma map_fst_with_names_from (c:ctx) (s : list exp)
+  : size s = size c -> map fst (with_names_from c s) = map fst c.
+Proof using .
+  elim: c s; intros until s; case: s; intros; break;simpl in *; auto.
+  { inversion H0. }
+  {
+    f_equal; auto.
+  }
+Qed.
+
+Lemma map_snd_with_names_from  (c:ctx) (s : list exp)
+  : size s = size c -> map snd (with_names_from c s) = s.
+Proof using .
+  elim: c s; intros until s; case: s; intros; break;simpl in *; auto.
+  { inversion H. }
+  {
+    f_equal; auto.
+  }
+Qed.
